# Amplificador no inversor "Mejor nodos"

$$
I_1 - I_2 = 0
$$

$$
\frac{e_0 - V_x}{R_2} - \frac{V_x - 0}{R_1} = 0
$$

$$
V_x = e_i
$$

$$
\frac{e_0 - e_i}{R_2} - \frac{e_i}{R_1} = 0
$$

$$
e_0 = e_i \left( \frac{1}{R_2} + \frac{1}{R_1} \right) R_2 \Rightarrow e_0 = e_i \left( 1 + \frac{R_2}{R_1} \right)
$$

# Con elementos almacenadores de energ√≠a

$$
i_1 - i_2 - i_3 = 0
$$

$$
\frac{e_i - e'}{R_1} - \frac{e' - e_0}{R_2} - C \frac{d(e' - e_0)}{dt} = 0
$$

$$
e' = 0
$$

$$
\frac{e_i}{R_1} - \frac{-e_0}{R_2} - C \frac{d(-e_0)}{dt} = 0
$$

$$
\frac{e_i}{R_1} = -\frac{e_0}{R_2} - C \frac{d(e_0)}{dt}
$$

## Actividad

$$
i_1 + i_2 - i_3 = i_4 = 0
$$

$$
E_i - V_x \Rightarrow \text{multi}
$$

$$
e_i \frac{d(E_i - V_x)}{dt} + \frac{E_i - V_x}{R_1} - \frac{R_2 \, dV_x - E}{dt} - \frac{V_x - E}{R_2} = 0
$$

$$
V_x = 0
$$

$$
e_i \frac{dE_i}{dt} + \frac{E_i}{R_1} + L_2 \frac{dE}{dt} + \frac{E}{R_2} = 0
$$
